moving minGap to the defn of a CPS, where it should belong. This will help getting rid of the explicit ugly minGap parameter required at many places.

src/CPS.v
@@ -315,14 +315,28 @@ Definition SwSemantics
 Record MessageDeliveryParams :=
 { expectedDelay : option QTime; maxVariation : QTime}.
 
+(* 
+An advantage to using a typeclass instead of the desugared record is that
+[minGap] gets automatically resolved to the CPS instance in scope,
+thus promoting brevity.
+*)
 Class CPS (RosLoc: Type) 
      {rldeq : DecEq RosLoc} :=
 {
+(* TODO : rename to nodeSemantics *)
    locNode: RosLoc -> NodeSemantics;
 
    validTopics : RosLoc -> (@TopicInfo RosTopic);
 
-   accDelDelay : RosLoc -> RosLoc -> Q -> Prop
+   accDelDelay : RosLoc -> RosLoc -> Q -> Prop;
+
+(** 
+The minimum gap between two events is constrained by the speed of the hardware,
+e.g. the NIC. Hence, it has to be specified while defining the CPS 
+*)
+  minGap : Q;
+  (* remove this and change the type of [minGap] to [Qpos] *)
+  minGapPos : (0 < minGap)%Q
 }.
 
 
@@ -333,10 +347,18 @@ Set Implicit Arguments.
 
 Arguments well_founded {A} P.
 
+(* 
+Currently, all we need from the CPS instance is the value of minGap.
+In future, a definition of CPS might put addiditonal consraints on the event ordering
+*)
 Class EventOrdering 
-   {Topic Event Loc: Type} (minGap:Q)
-  `{rtopic : TopicClass Topic} 
-  `{etype : @EventType _ _ _ Event tdeq} :=
+{PhysicalEnvType Topic Event Loc  : Type}
+  {tdeq : DecEq Topic}
+  {edeq : DecEq Event}
+  {ldeq : DecEq Loc}
+  {rtopic : @TopicClass Topic tdeq} 
+  {etype : @EventType Topic tdeq rtopic Event edeq} 
+  {rlct : @CPS PhysicalEnvType Topic tdeq rtopic Loc ldeq} :=
 {
   eLoc : Event ->  Loc;
 
@@ -366,9 +388,6 @@ Class EventOrdering
     /\ (eLoc e1 = eLoc e2 
         -> minGap <= (Qabs ((eTime e1) - (eTime e2))))%Q;
 
-  (* remove this and change the type of [minGap] to [Qpos] *)
-  minGapPos : (0 < minGap)%Q;
-
   (* While this definitely a sensible property, is it needed anywhere? *)
   uniqueSendInfo :
     ∀ (si : SendEvtInfo) ev1 ev2,
@@ -395,23 +414,21 @@ Class EventOrdering
     causalWf : well_founded  causedBy
 }.
 
-Definition PossibleSendRecvPair (minGap:Q)
+Definition PossibleSendRecvPair
   {Topic Event Loc PhysicalEnvType : Type}
   {tdeq : DecEq Topic}
   {edeq : DecEq Event}
   {ldeq : DecEq Loc}
   {rtopic : @TopicClass Topic tdeq} 
   {etype : @EventType Topic tdeq rtopic Event edeq} 
-  {_ : @EventOrdering Topic Event Loc minGap tdeq rtopic edeq etype}
   {rlct : @CPS PhysicalEnvType Topic tdeq rtopic Loc ldeq}
+  {eo : @EventOrdering PhysicalEnvType Topic Event Loc tdeq edeq ldeq rtopic  etype rlct}
   (Es  Er : Event) : Prop
  :=
    (fst (eMesg Es) = fst (eMesg Er))
    /\ (validRecvMesg (validTopics (eLoc Er)) (eMesg Er))
    /\ (validSendMesg (validTopics (eLoc Es)) (eMesg Es))
    /\ (accDelDelay  (eLoc Es) (eLoc Er) (eTime Er - eTime Es)).
-
-
 
 
 Record EOReliableDelivery (minGap:Q)
@@ -421,8 +438,9 @@ Record EOReliableDelivery (minGap:Q)
   {ldeq : DecEq Loc}
   {rtopic : @TopicClass Topic tdeq} 
   {etype : @EventType Topic tdeq rtopic Event edeq} 
-  {eo : @EventOrdering Topic Event Loc minGap tdeq rtopic edeq etype}
-  {rlct : @CPS PhysicalEnvType Topic tdeq rtopic  Loc ldeq} :=
+  {rlct : @CPS PhysicalEnvType Topic tdeq rtopic  Loc ldeq}
+  {eo : @EventOrdering PhysicalEnvType Topic Event Loc  tdeq edeq ldeq rtopic  etype rlct}
+ :=
 {
     eventualDelivery: forall (Es : Event),
           isSendEvt Es
@@ -457,7 +475,7 @@ Context  (minGap:Q)
   {tdeq : DecEq Topic}
   {ldeq : DecEq Loc}
   {rtopic : @TopicClass Topic tdeq} 
-  {rlct : @CPS PhysicalEvType Topic tdeq rtopic  Loc ldeq}.
+  {cps : @CPS PhysicalEvType Topic tdeq rtopic  Loc ldeq}.
 
 Close Scope Q_scope.
 
@@ -475,7 +493,7 @@ Record CPSExecution  := {
   CPSEvent : Type;
   CPSedeq : DecEq CPSEvent;
   CPSetype : @EventType Topic tdeq rtopic CPSEvent CPSedeq;
-  CPSEventOrdering : @EventOrdering Topic CPSEvent Loc minGap tdeq rtopic CPSedeq CPSetype;
+  CPSEventOrdering : @EventOrdering PhysicalEvType Topic CPSEvent Loc tdeq CPSedeq ldeq rtopic CPSetype cps;
   CPSAgentSpecsHold : ∀l:Loc, (locNode l) CPSEvent CPSedeq CPSetype physicsEvolution (localEvts l)
 }.
 
@@ -491,7 +509,7 @@ Global Instance EventTypeInstanceCPSEvent : @EventType Topic tdeq
    rtopic (CPSEvent ce) (CPSedeq ce) 
   := CPSetype  ce.
 Global Instance EventOrderingnInstanceCPSEvent : 
-  @EventOrdering Topic (CPSEvent ce) Loc minGap tdeq rtopic (CPSedeq ce) (CPSetype ce)
+  @EventOrdering PhysicalEvType Topic (CPSEvent ce) Loc tdeq (CPSedeq ce) ldeq  rtopic (CPSetype ce) cps
   := CPSEventOrdering  ce.
 
 End CPSExecutionTypeclasses.
